lemmas, types

src/dafny/BinaryOperations.dfy
@@ -7,80 +7,195 @@
 
 module {:options "-functionSyntax:4"} BinaryOperations {
 
-  ghost predicate Associative<T(!new)>(bop: (T, T) -> T) {
+  ghost predicate IsAssociative<T(!new)>(bop: (T, T) -> T) {
     forall x, y, z :: bop(bop(x, y), z) == bop(x, bop(y, z))
   }
 
-  ghost predicate UnitalLeft<T(!new)>(bop: (T, T) -> T, unit: T) {
+  ghost predicate IsLeftUnital<T(!new)>(bop: (T, T) -> T, unit: T) {
     forall x :: bop(unit, x) == x
   }
 
-  ghost predicate UnitalRight<T(!new)>(bop: (T, T) -> T, unit: T) {
+  ghost predicate IsRightUnital<T(!new)>(bop: (T, T) -> T, unit: T) {
     forall x :: bop(x, unit) == x
   }
 
-  ghost predicate Unital<T(!new)>(bop: (T, T) -> T, unit: T) {
-    && UnitalLeft(bop, unit)
-    && UnitalRight(bop, unit)
+  ghost predicate IsUnital<T(!new)>(bop: (T, T) -> T, unit: T) {
+    && IsLeftUnital(bop, unit)
+    && IsRightUnital(bop, unit)
   }
 
-  ghost predicate InverseLeft<T(!new)>(bop: (T, T) -> T, inverse: T --> T, unit: T) {
+  ghost predicate IsLeftInverse<T(!new)>(bop: (T, T) -> T, inverse: T --> T, unit: T) {
     forall x | inverse.requires(x) :: bop(inverse(x), x) == unit
   }
 
-  ghost predicate InverseRight<T(!new)>(bop: (T, T) -> T, inverse: T --> T, unit: T) {
+  ghost predicate IsRightInverse<T(!new)>(bop: (T, T) -> T, inverse: T --> T, unit: T) {
     forall x | inverse.requires(x) :: bop(x, inverse(x)) == unit
   }
 
-  ghost predicate Inverse<T(!new)>(bop: (T, T) -> T, inverse: T --> T, unit: T) {
-    && InverseLeft(bop, inverse, unit)
-    && InverseRight(bop, inverse, unit)
+  ghost predicate IsInverse<T(!new)>(bop: (T, T) -> T, inverse: T --> T, unit: T) {
+    && IsLeftInverse(bop, inverse, unit)
+    && IsRightInverse(bop, inverse, unit)
   }
 
-  ghost predicate Abelian<T(!new)>(bop: (T, T) -> T) {
+  ghost predicate IsAbelian<T(!new)>(bop: (T, T) -> T) {
     forall x, y :: bop(x, y) == bop(y, x)
   }
 
-  ghost predicate DistributiveRight<T(!new)>(bop1: (T, T) -> T, bop2: (T, T) -> T) {
+  ghost predicate IsRightDistributive<T(!new)>(bop1: (T, T) -> T, bop2: (T, T) -> T) {
     forall x, y, z :: bop2(bop1(x, y), z) == bop1(bop2(x, z), bop2(y, z))
   }
 
-  ghost predicate DistributiveLeft<T(!new)>(bop1: (T, T) -> T, bop2: (T, T) -> T) {
+  ghost predicate IsLeftDistributive<T(!new)>(bop1: (T, T) -> T, bop2: (T, T) -> T) {
     forall x, y, z :: bop2(x, bop1(y, z)) == bop1(bop2(x, y), bop2(x, z))
   }
 
-  ghost predicate Distributive<T(!new)>(bop1: (T, T) -> T, bop2: (T, T) -> T) {
-    && DistributiveLeft(bop1, bop2)
-    && DistributiveRight(bop1, bop2)
+  ghost predicate IsDistributive<T(!new)>(bop1: (T, T) -> T, bop2: (T, T) -> T) {
+    && IsLeftDistributive(bop1, bop2)
+    && IsRightDistributive(bop1, bop2)
   }
 
-  ghost predicate Monoid<T(!new)>(bop: (T, T) -> T, unit: T) {
-    && Associative(bop)
-    && Unital(bop, unit)
+  ghost predicate IsMonoid<T(!new)>(bop: (T, T) -> T, unit: T) {
+    && IsAssociative(bop)
+    && IsUnital(bop, unit)
   }
 
-  ghost predicate Group<T(!new)>(bop: (T, T) -> T, inverse: T --> T, unit: T) {
-    && Monoid(bop, unit)
-    && Inverse(bop, inverse, unit)
+  datatype MonoidStructure<!T(!new)> = MonoidStructure(bop: (T, T) -> T, unit: T)
+  type Monoid<!T(!new)> = g: MonoidStructure | IsMonoid(g.bop, g.unit) witness *
+
+  ghost predicate IsGroup<T(!new)>(bop: (T, T) -> T, inverse: T --> T, unit: T) {
+    && IsMonoid(bop, unit)
+    && IsInverse(bop, inverse, unit)
   }
 
-  ghost predicate AbelianGroup<T(!new)>(bop: (T, T) -> T, inverse: T --> T, unit: T) {
-    && Group(bop, inverse, unit)
-    && Abelian(bop)
+  datatype GroupStructure<!T(!new)> = GroupStructure(bop: (T, T) -> T, inverse: T -> T, unit: T)
+  type Group<!T(!new)> = g: GroupStructure | IsGroup(g.bop, g.inverse, g.unit) witness *
+
+  ghost predicate IsAbelianGroup<T(!new)>(bop: (T, T) -> T, inverse: T --> T, unit: T) {
+    && IsGroup(bop, inverse, unit)
+    && IsAbelian(bop)
   }
 
-  ghost predicate Ring<T(!new)>(add: (T, T) -> T, minus: T -> T, zero: T, mult: (T, T) -> T, one: T) {
-    && AbelianGroup(add, minus, zero)
-    && Monoid(mult, one)
-    && Distributive(add, mult)
+  type AbelianGroup<!T(!new)> = g: GroupStructure | IsAbelianGroup(g.bop, g.inverse, g.unit) witness *
+
+  ghost predicate IsRing<T(!new)>(add: (T, T) -> T, minus: T -> T, zero: T, mult: (T, T) -> T, one: T) {
+    && IsAbelianGroup(add, minus, zero)
+    && IsMonoid(mult, one)
+    && IsDistributive(add, mult)
   }
 
-  ghost predicate Field<T(!new)>(add: (T, T) -> T, minus: T -> T, zero: T, mult: (T, T) -> T, div: T --> T, one: T)
+  datatype RingStructure<!T(!new)> = RingStructure(add: (T, T) -> T, minus: T -> T, zero: T, mult: (T, T) -> T, one: T)
+  type Ring<!T(!new)> = r: RingStructure | IsRing(r.add, r.minus, r.zero, r.mult, r.one) witness *
+
+  ghost predicate IsField<T(!new)>(add: (T, T) -> T, minus: T -> T, zero: T, mult: (T, T) -> T, div: T --> T, one: T)
     requires forall t :: (t != zero) ==> div.requires(t)
   {
-    && AbelianGroup(add, minus, zero)
-    && AbelianGroup(mult, div, one)
-    && DistributiveLeft(add, mult)
+    && IsAbelianGroup(add, minus, zero)
+    && IsAbelianGroup(mult, div, one)
+    && IsLeftDistributive(add, mult)
+  }
+
+  datatype FieldStructure<!T(!new)> = RingStructure(add: (T, T) -> T, minus: T -> T, zero: T, mult: (T, T) -> T, div: T --> T, one: T)
+  type FieldPre<!T(!new)> = f: FieldStructure | (forall t :: (t != f.zero) ==> f.div.requires(t)) witness *
+  type Field<!T(!new)> = f: FieldPre | IsField(f.add, f.minus, f.zero, f.mult, f.div, f.one) witness *
+
+  ghost predicate IsHomomorphism<S(!new),T>(bop1: (S, S) -> S, bop2: (T, T) -> T, f: S -> T) {
+    forall x, y :: f(bop1(x, y)) == bop2(f(x), f(y))
+  }
+
+  lemma MonoidInverseIsUnique<T(!new)>(bop: (T, T) -> T, inverse1: T -> T, inverse2: T -> T, unit: T)
+    requires IsMonoid(bop, unit)
+    requires IsInverse(bop, inverse1, unit)
+    requires IsInverse(bop, inverse2, unit)
+    ensures forall x :: inverse1(x) == inverse2(x)
+  {
+    forall x ensures inverse1(x) == inverse2(x) {
+      calc {
+        inverse1(x);
+      == { assert IsRightUnital(bop, unit); }
+        bop(inverse1(x), unit);
+      == { assert IsRightInverse(bop, inverse2, unit); assert unit == bop(x, inverse2(x)); }
+        bop(inverse1(x), bop(x, inverse2(x)));
+      == { assert IsAssociative(bop); }
+        bop(bop(inverse1(x), x), inverse2(x));
+      == { assert IsLeftInverse(bop, inverse1, unit); assert bop(inverse1(x), x) == unit;}
+        bop(unit, inverse2(x));
+      == { assert IsLeftUnital(bop, unit); }
+        inverse2(x);
+      }
+    }
+  }
+
+  lemma UnitIsUnique<T(!new)>(bop: (T, T) -> T, unit1: T, unit2: T)
+    requires IsUnital(bop, unit1)
+    requires IsUnital(bop, unit2)
+    ensures unit1 == unit2
+  {
+    calc {
+      unit1;
+    == { assert IsRightUnital(bop, unit2); }
+      bop(unit1, unit2);
+    == { assert IsLeftUnital(bop, unit1); }
+      unit2;
+    }
+  }
+
+
+  lemma UnitIsSelfInverse<T(!new)>(g: Group<T>)
+    ensures g.unit == g.inverse(g.unit)
+  {
+    calc {
+      g.unit;
+    == { assert IsLeftInverse(g.bop, g.inverse, g.unit); }
+      g.bop(g.inverse(g.unit), g.unit);
+    == { assert IsRightUnital(g.bop, g.unit); }
+      g.inverse(g.unit);
+    }
+  }
+
+  lemma GroupHomomorphismPreservesUnit<S(!new),T(!new)>(g1: Group<S>, g2: Group<T>, f: S -> T)
+    requires IsHomomorphism(g1.bop, g2.bop, f)
+    ensures f(g1.unit) == g2.unit
+  {
+    calc {
+      f(g1.unit);
+    == { assert IsRightUnital(g2.bop, g2.unit); }
+      g2.bop(f(g1.unit), g2.unit);
+    == { assert IsRightInverse(g2.bop, g2.inverse, g2.unit); assert g2.unit ==  g2.bop(f(g1.unit), g2.inverse(f(g1.unit))); }
+      g2.bop(f(g1.unit), g2.bop(f(g1.unit), g2.inverse(f(g1.unit))));
+    == { assert IsAssociative(g2.bop); }
+      g2.bop(g2.bop(f(g1.unit), f(g1.unit)), g2.inverse(f(g1.unit)));
+    == { assert IsHomomorphism(g1.bop, g2.bop, f); assert g2.bop(f(g1.unit), f(g1.unit)) == f(g1.bop(g1.unit, g1.unit)); }
+      g2.bop(f(g1.bop(g1.unit, g1.unit)), g2.inverse(f(g1.unit)));
+    == { assert IsLeftUnital(g1.bop, g1.unit); assert g1.bop(g1.unit, g1.unit) == g1.unit; }
+      g2.bop(f(g1.unit), g2.inverse(f(g1.unit)));
+    == { assert IsRightInverse(g2.bop, g2.inverse, g2.unit); }
+      g2.unit;
+    }
+  }
+
+  lemma GroupHomomorphismPreservesInverse<S(!new),T(!new)>(g1: Group<S>, g2: Group<T>, f: S -> T)
+    requires IsHomomorphism(g1.bop, g2.bop, f)
+    ensures forall x :: f(g1.inverse(x)) == g2.inverse(f(x))
+  {
+    forall x ensures f(g1.inverse(x)) == g2.inverse(f(x)) {
+      calc {
+        f(g1.inverse(x));
+      == { assert IsRightUnital(g2.bop, g2.unit); }
+        g2.bop(f(g1.inverse(x)), g2.unit);
+      == { assert IsRightInverse(g2.bop, g2.inverse, g2.unit); assert g2.unit == g2.bop(f(x), g2.inverse(f(x))); }
+        g2.bop(f(g1.inverse(x)), g2.bop(f(x), g2.inverse(f(x))));
+      == { assert IsAssociative(g2.bop); }
+        g2.bop(g2.bop(f(g1.inverse(x)), f(x)), g2.inverse(f(x)));
+      == { assert IsHomomorphism(g1.bop, g2.bop, f); assert g2.bop(f(g1.inverse(x)), f(x)) == f(g1.bop(g1.inverse(x), x)); }
+        g2.bop(f(g1.bop(g1.inverse(x), x)), g2.inverse(f(x)));
+      == { assert IsLeftInverse(g1.bop, g1.inverse, g1.unit); assert g1.bop(g1.inverse(x), x) == g1.unit; }
+        g2.bop(f(g1.unit), g2.inverse(f(x)));
+      == { GroupHomomorphismPreservesUnit(g1, g2, f); assert f(g1.unit) == g2.unit; }
+        g2.bop(g2.unit, g2.inverse(f(x)));
+      == { assert IsLeftUnital(g2.bop, g2.unit); }
+        g2.inverse(f(x));
+      }
+    }
   }
 
 }
